CODIGO/SUMA/Transformations/ParticionToEnvasar.dfy
@@ -1,10 +1,49 @@
 include "../Auxiliar/Sum.dfy"
-include "../Problems/Suma.dfy"
 include "../Problems/Particion.dfy"
+include "../Problems/Envasar.dfy"
 
 
-function Particion_to_Envasar(A:multiset<int>) : (r:(multiset<int>, int, int))
+function Particion_to_Envasar(A:multiset<nat>) : (r:(multiset<nat>, nat, nat))
 {
     var S := FSum(A)/2;
-    (A, S,2)
+    (A,S,2)
+}
+
+lemma Particion_Envasar(A:multiset<nat>)
+  ensures var (EA,EE,Ek) := Particion_to_Envasar(A);
+          Particion(A) <==> Envasar(EA,EE,Ek)
+{ 
+    Particion_Envasar1(A);
+    Particion_Envasar2(A);
+}
+
+lemma Particion_Envasar1(A:multiset<nat>)
+    ensures var (EA,EE,Ek) := Particion_to_Envasar(A);
+          Particion(A) <== Envasar(EA,EE,Ek)
+{   
+    // EA = {1, 2, 3}, EE = 3, Ek = 2
+    var (EA,EE,Ek) := Particion_to_Envasar(A);
+    if (Envasar(EA,EE,Ek)) {
+        var C: multiset<multiset<nat>> :| forall e | e in C :: e <= EA && GSum(e) <= EE && |C| <= Ek; // C = { {1,2}, {3}}
+        var P1 :| P1 in C; // P1 = {1,2}
+        C := C - multiset{P1}; 
+        var P2 :| P2 in C; // P2 = {3}
+
+        assert P1 in C && P2 in C && P1 != P2 && P1 * P2 == multiset{} && P1 + P2 == A && GSum(P1) == GSum(P2); // P1 y P2 son una particion de A?
+    }
+}
+
+
+lemma Particion_Envasar2(A:multiset<nat>)
+    ensures var (EA,EE,Ek) := Particion_to_Envasar(A);
+          Particion(A) ==> Envasar(EA,EE,Ek)
+{
+    // A = {1, 2, 3}
+    if (Particion(A)) {
+        var (EA,EE,Ek) := Particion_to_Envasar(A);
+
+        var P1:multiset<nat>, P2:multiset<nat> :| P1 <= A && P2 <= A && P1 * P2 == multiset{} && P1 + P2 == A && GSum(P1) == GSum(P2); // {1,2} {3}
+        var C: multiset<multiset<nat>> := multiset{P1, P2}; // { {1,2}, {3}}
+        assert forall e1 | e1 in C :: (e1 <= A && GSum(e1) <= E && forall e2 | e2 in I :: e1 * e2 == multiset{}) :: |I| <= k && Union(I) == A;
+    }
 }
