CODIGO/SUMA/Transformations/SumaToIntervalo.dfy
@@ -3,12 +3,12 @@ include "../Problems/Suma.dfy"
 include "../Problems/Intervalo.dfy"
 
 
-function Suma_To_Intervalo(A:multiset<nat>, S:nat) : (r:(multiset<nat>, nat, nat))
+function Suma_To_Intervalo(A:multiset<int>, S:int) : (r:(multiset<int>, int, int))
 {
     (A, S, S+1)
 }
 
-lemma Suma_Intervalo(A:multiset<nat>, S:nat)
+lemma Suma_Intervalo(A:multiset<int>, S:int)
   ensures var (IE,IS,IT) := Suma_To_Intervalo(A, S);
           Suma(A,S) <==> Intervalo(IE,IS,IT)
 { 
@@ -16,19 +16,19 @@ lemma Suma_Intervalo(A:multiset<nat>, S:nat)
     Suma_Intervalo2(A,S);
 }
 
-lemma Suma_Intervalo1(A:multiset<nat>, S:nat)
+lemma Suma_Intervalo1(A:multiset<int>, S:int)
     ensures var (IE,IS,IT) := Suma_To_Intervalo(A, S);
           Suma(A,S) <== Intervalo(IE,IS,IT)
 {   
     var (IE,IS,IT) := Suma_To_Intervalo(A,S);
     // IE = {1, 2, 4}, IS = 6, IT = 7
     if (Intervalo(IE,IS,IT)) {
-        var C:multiset<nat> :| C <= A && IS <= GSum(C) < IT; // C = 2, 4
+        var C:multiset<int> :| C <= A && IS <= GSum(C) < IT; // C = 2, 4  ->  Sum(C) = 6
         assert GSum(C) == S; // Sum(C) == 6
     }
 }
 
-lemma Suma_Intervalo2(A:multiset<nat>, S:nat)
+lemma Suma_Intervalo2(A:multiset<int>, S:int)
     ensures var (IE,IS,IT) := Suma_To_Intervalo(A,S);
           Suma(A,S) ==> Intervalo(IE,IS,IT)
 {
@@ -36,7 +36,7 @@ lemma Suma_Intervalo2(A:multiset<nat>, S:nat)
     if (Suma(A,S)) {
         var (IE,IS,IT) := Suma_To_Intervalo(A,S);
 
-        var C:multiset<nat> :| C <= A && GSum(C) == S; // C = 2, 4  ->  Sum(C) = 6
+        var C:multiset<int> :| C <= A && GSum(C) == S; // C = 2, 4  ->  Sum(C) = 6
         assert IS <= GSum(C) < IT; // IS <= 6 < IT
     }
 }
