CODIGO/SUMA/Transformations/SumaToParticion.dfy
@@ -8,3 +8,36 @@ function Suma_to_Particion(A:multiset<int>, S:int) : (r:(multiset<int>))
     var N := 2*S - FSum(A);
     (A + multiset{N})
 }
+
+lemma Suma_Particion(A:multiset<int>, S:int)
+  ensures var (PA) := Suma_to_Particion(A, S);
+          Suma(A,S) <==> Particion(PA)
+{ 
+    Suma_Particion1(A,S);
+    Suma_Particion2(A,S);
+}
+
+lemma Suma_Particion1(A:multiset<int>, S:int)
+    ensures var (PA) := Suma_to_Particion(A, S);
+          Suma(A,S) <== Particion(PA)
+{   
+    var (PA) := Suma_To_Intervalo(A,S);
+    // PA = {1, 2, 3, 4, 2(N)}
+    if (Particion(PA)) {
+        var C:multiset<int> :| C <= A && IS <= GSum(C) < IT; // C = 2, 4  ->  Sum(C) = 6
+        assert GSum(C) == S; // Sum(C) == 6
+    }
+}
+
+lemma Suma_Particion2(A:multiset<int>, S:int)
+    ensures var (PA) := Suma_to_Particion(A, S);
+          Suma(A,S) ==> Particion(PA)
+{
+    // A = {1, 2, 4}, S = 6
+    if (Suma(A,S)) {
+        var (PA) := Suma_To_Intervalo(A,S);
+
+        var C:multiset<int> :| C <= A && GSum(C) == S; // C = 2, 4  ->  Sum(C) = 6
+        assert IS <= GSum(C) < IT; // IS <= 6 < IT
+    }
+}
